verification/semantics/lisp_ir/LispIR.CompilerCorrectnessArith.fst
@@ -1,0 +1,111 @@
+module LispIR.CompilerCorrectnessArith
+open FStar.Pervasives
+open FStar.List.Tot
+
+type arith_expr =
+  | ANum of int
+  | AAdd of arith_expr * arith_expr
+  | ASub of arith_expr * arith_expr
+  | ANeg of arith_expr
+  | AMul of arith_expr * arith_expr
+
+type arith_op =
+  | Push of int
+  | OpAdd
+  | OpSub
+  | OpNeg
+  | OpMul
+
+val arith_compile : arith_expr -> list arith_op
+let rec arith_compile = function
+  | ANum n -> [Push n]
+  | AAdd (a, b) -> arith_compile a @ arith_compile b @ [OpAdd]
+  | ASub (a, b) -> arith_compile a @ arith_compile b @ [OpSub]
+  | ANeg a -> arith_compile a @ [OpNeg]
+  | AMul (a, b) -> arith_compile a @ arith_compile b @ [OpMul]
+
+val arith_eval : arith_expr -> int
+let rec arith_eval = function
+  | ANum n -> n
+  | AAdd (a, b) -> arith_eval a + arith_eval b
+  | ASub (a, b) -> arith_eval a - arith_eval b
+  | ANeg a -> 0 - arith_eval a
+  | AMul (a, b) -> Prims.op_Multiply (arith_eval a) (arith_eval b)
+
+val arith_vm : fuel:int -> code:list arith_op -> stack:list int ->
+  Tot (list int * int) (decreases fuel)
+let rec arith_vm fuel code stack =
+  if fuel <= 0 then (stack, fuel)
+  else match code with
+  | [] -> (stack, fuel)
+  | Push n :: rest -> arith_vm (fuel - 1) rest (n :: stack)
+  | OpAdd :: rest ->
+    (match stack with
+     | a :: b :: stk' -> arith_vm (fuel - 1) rest ((b + a) :: stk')
+     | _ -> (stack, 0))
+  | OpSub :: rest ->
+    (match stack with
+     | a :: b :: stk' -> arith_vm (fuel - 1) rest ((b - a) :: stk')
+     | _ -> (stack, 0))
+  | OpNeg :: rest ->
+    (match stack with
+     | a :: stk' -> arith_vm (fuel - 1) rest ((0 - a) :: stk')
+     | _ -> (stack, 0))
+  | OpMul :: rest ->
+    (match stack with
+     | a :: b :: stk' -> arith_vm (fuel - 1) rest (Prims.op_Multiply b a :: stk')
+     | _ -> (stack, 0))
+
+val run_then : fuel:int -> c1:list arith_op -> s:list int ->
+  c2:list arith_op -> Tot (list int * int)
+let run_then fuel c1 s c2 =
+  let (s1, f1) = arith_vm fuel c1 s in
+  arith_vm f1 c2 s1
+
+val arith_vm_sequential : c1:list arith_op -> fuel:int -> c2:list arith_op -> s:list int ->
+  Lemma (ensures arith_vm fuel (c1 @ c2) s = run_then fuel c1 s c2)
+let rec arith_vm_sequential c1 fuel c2 s =
+  match c1 with
+  | [] -> ()
+  | Push n :: rest -> arith_vm_sequential rest (fuel - 1) c2 (n :: s)
+  | OpAdd :: rest ->
+    (match s with
+     | a :: b :: stk' -> arith_vm_sequential rest (fuel - 1) c2 ((b + a) :: stk')
+     | _ -> ())
+  | OpSub :: rest ->
+    (match s with
+     | a :: b :: stk' -> arith_vm_sequential rest (fuel - 1) c2 ((b - a) :: stk')
+     | _ -> ())
+  | OpNeg :: rest ->
+    (match s with
+     | a :: stk' -> arith_vm_sequential rest (fuel - 1) c2 ((0 - a) :: stk')
+     | _ -> ())
+  | OpMul :: rest ->
+    (match s with
+     | a :: b :: stk' -> arith_vm_sequential rest (fuel - 1) c2 (Prims.op_Multiply b a :: stk')
+     | _ -> ())
+
+val get_stack : r:list int * int -> list int
+let get_stack (s, _) = s
+
+val arith_compiler_correctness : fuel:int -> e:arith_expr -> Lemma
+  (get_stack (arith_vm fuel (arith_compile e) []) = [arith_eval e])
+let rec arith_compiler_correctness fuel e =
+  match e with
+  | ANum _ -> ()
+  | AAdd (a, b) ->
+    arith_compiler_correctness fuel a;
+    arith_compiler_correctness fuel b;
+    arith_vm_sequential (arith_compile a) fuel (arith_compile b @ [OpAdd]) []
+  | ASub (a, b) ->
+    arith_compiler_correctness fuel a;
+    arith_compiler_correctness fuel b;
+    arith_vm_sequential (arith_compile a) fuel (arith_compile b @ [OpSub]) []
+  | ANeg a ->
+    arith_compiler_correctness fuel a;
+    arith_vm_sequential (arith_compile a) fuel [OpNeg] []
+  | AMul (a, b) ->
+    arith_compiler_correctness fuel a;
+    arith_compiler_correctness fuel b;
+    arith_vm_sequential (arith_compile a) fuel (arith_compile b @ [OpMul]) []
+
