verification/tests/TestNorm.fst
@@ -1,0 +1,30 @@
+module TestNorm
+
+open FStar.Seq
+open FStar.Seq.Base
+open Lisp.Types
+open Lisp.Values
+open Lisp.Compiler
+
+// Test 1: does normalizer unfold vec_len (Vec (create 1 (Num 0)))?
+val test1 : unit -> Lemma
+  (vec_len (Vec (create 1 (Num 0))) = 1)
+let test1 () =
+  assert_norm (vec_len (Vec (create 1 (Num 0))) = 1)
+
+// Test 2: does normalizer unfold length (create 1 (Num 0))?
+val test2 : unit -> Lemma
+  (length (create 1 (Num 0)) = 1)
+let test2 () =
+  assert_norm (length (create 1 (Num 0)) = 1)
+
+// Test 3: does normalizer unfold length (append (create 1 (Num 0)) (create 1 (Num 1)))?
+val test3 : unit -> Lemma
+  (length (append (create 1 (Num 0)) (create 1 (Num 1))) = 2)
+let test3 () =
+  assert_norm (length (append (create 1 (Num 0)) (create 1 (Num 1))) = 2)
+
+// Test 4: does SMT prove length (append s (create 1 x)) = length s + 1?
+val test4 : s:seq lisp_val -> x:lisp_val -> Lemma
+  (length (append s (create 1 x)) = length s + 1)
+let test4 s x = ()
