verification/tests/TestVecConj.fst
@@ -1,0 +1,50 @@
+module TestVecConj
+
+open FStar.Seq
+open FStar.Seq.Base
+open Lisp.Types
+open Lisp.Values
+open Lisp.Compiler
+
+val opt_is_none : option lisp_val -> Tot bool
+let opt_is_none o = match o with | None -> true | Some _ -> false
+
+val opt_is_some : option lisp_val -> Tot bool
+let opt_is_some o = match o with | Some _ -> true | None -> false
+
+val my_conj : lisp_val -> lisp_val -> Tot lisp_val
+let my_conj x v =
+  match v with
+  | Vec s -> Vec (append s (create 1 x))
+  | _ -> Vec (create 1 x)
+
+val my_len : lisp_val -> Tot int
+let my_len v =
+  match v with
+  | Vec s -> length s
+  | _ -> 0
+
+// Soundness: local mirrors agree with Lisp.Values for Vec inputs
+val conj_sound : s:seq lisp_val -> x:lisp_val -> Lemma
+  (match my_conj x (Vec s), vec_conj x (Vec s) with
+   | Vec a, Vec b -> length a = length b
+   | _ -> true)
+let conj_sound s x =
+  assert_norm (match my_conj x (Vec s), vec_conj x (Vec s) with
+               | Vec a, Vec b -> length a = length b
+               | _ -> true)
+
+val len_sound : v:lisp_val -> Lemma
+  (match v with
+   | Vec s -> my_len v = vec_len v
+   | _ -> true)
+let len_sound v =
+  assert_norm (my_len v = vec_len v)
+
+// vec_conj increases length by 1
+val vec_conj_len : s:seq lisp_val -> x:lisp_val -> Lemma
+  (vec_len (vec_conj (Vec s) x) = length s + 1)
+let vec_conj_len s x =
+  conj_sound s x;
+  len_sound (my_conj x (Vec s));
+  ()
